***Definitions***: $U$ represents  the domain for the predicate
 - $\forall x. P(x) \equiv P(U_{1}) \land P(U_{2}) \land P(U_{3}) \land ... \land P(U_{n})$ 
 - $\exists x. P(x) \equiv P(U_{1}) \lor P(U_{2}) \lor P(U_{3}) \lor ... \lor P(U_{n})$ 
 - $\neg \forall x. P(x) \equiv \exists x. \neg P(x)$
 - $\neg \exists x. P(x) \equiv \forall x. \neg P(x)$

##### Question 8
Domain: $U = -2, -1, 0, 1, 2$
1. $\forall x. \neg P(x)$ 
	$\equiv \neg \exists x. P(x)$ 
	$\equiv \neg (P(-2) \lor P(-1) \lor P(0) \lor P(1) \lor P(2))$
	$\equiv \neg P(-2) \land \neg P(-1) \land \neg P(0) \land \neg P(1) \land \neg P(2)$ 
2. $\forall x. P(x)$
	$\equiv P(-2) \land P(-1) \land P(0) \land P(1) \land P(2)$
3. $\neg \forall x. P(x)$
	$\equiv \neg (P(-2) \land P(-1) \land P(0) \land P(1) \land P(2))$
	$\equiv \neg P(-2) \lor \neg P(-1) \lor \neg P(0) \lor \neg P(1) \lor \neg P(2)$
4. $\exists x. \neg P(x)$
	$\equiv \neg \forall x. P(x)$
	$\equiv \neg (P(-2) \land P(-1) \land P(0) \land P(1) \land P(2))$
	$\equiv \neg P(-2) \lor \neg P(-1) \lor \neg P(0) \lor \neg P(1) \lor \neg P(2)$
5. $\exists x. P(x)$
	$\equiv P(-2) \lor P(-1) \lor P(0) \lor P(1) \lor P(2)$
6. $\neg \exists x. P(x)$
	$\equiv \neg (P(-2) \lor P(-1) \lor P(0) \lor P(1) \lor P(2))$
	$\equiv \neg P(-2) \land \neg P(-1) \land \neg P(0) \land \neg P(1) \land \neg P(2)$


##### Question 9






